rewrite complete

SingleUse.thy
@@ -2,8 +2,8 @@ theory SingleUse
   imports Main Setsum Update
 begin
 
-definition count_var :: "[('x::finite, 'b) update, 'x] \<Rightarrow> nat" where
-  "count_var f x \<equiv> \<Sum>y\<in>UNIV. count_list (f y) (Inl x)"
+definition count_var :: "[('x::finite, 'y::finite, 'b) update', 'y] \<Rightarrow> nat" where
+  "count_var f y0 \<equiv> \<Sum>y\<in>UNIV. count_list (f y) (Inl y0)"
 
 lemma "count_list (f y) (Inl x) \<le> count_var f x"
 proof -
@@ -14,10 +14,10 @@ proof -
     by (simp add: count_var_def)
 qed
 
-definition bounded :: "[nat, ('x::finite, 'b) update] \<Rightarrow> bool" where
-  "bounded k f = (\<forall>x. count_var f x \<le> k)"
+definition bounded :: "[nat, ('x::finite, 'y::finite, 'b) update'] \<Rightarrow> bool" where
+  "bounded k f \<equiv> (\<forall>y. count_var f y \<le> k)"
 
-abbreviation single_use  :: "(('x::finite, 'b) update) \<Rightarrow> bool" where
+abbreviation single_use  :: "(('x::finite, 'y::finite, 'b) update') \<Rightarrow> bool" where
   "single_use f \<equiv> bounded 1 f"
 
 lemma [simp]:  "count_list (xs@ys) a = count_list xs a + count_list ys a"
@@ -27,11 +27,10 @@ lemma [simp]:  "count_list (xs@ys) a = count_list xs a + count_list ys a"
 lemma sum_cong: "\<And>x. x\<in>A \<Longrightarrow> f = g \<Longrightarrow> sum f A = sum g A" by auto
 
 lemma basic_count: "count_list (hat_hom f xs) (Inl y) =
-                    (\<Sum>z\<in>UNIV. (count_list (f z) (Inl y) * count_list xs (Inl z)))"
+                    (\<Sum>z\<in>(UNIV::('a::finite) set). (count_list (f z) (Inl y) * count_list xs (Inl z)))"
 proof (induct xs rule: xa_induct)
   case Nil
-  show ?case
-    by (auto)
+  show ?case by simp
 next
   case (Alpha a xs) 
   then show ?case by simp
@@ -44,103 +43,82 @@ next
                    + (if x = z then count_list (f z) (Inl y) else 0))"
       by (rule sum_cong, auto)
     also have "... = (\<Sum>z\<in>UNIV. count_list (f z) (Inl y) * count_list xs (Inl z))
-                 + (\<Sum>z\<in>UNIV. if x = z then count_list (f z) (Inl y) else 0)"
+                      + (\<Sum>z\<in>UNIV. if x = z then count_list (f z) (Inl y) else 0)"
       by (rule sum.distrib)
     finally have "(\<Sum>z\<in>UNIV. count_list (f z) (Inl y) * (if x = z then count_list xs (Inl z) + 1 
-                                                          else count_list xs (Inl z)))
+                                                                  else count_list xs (Inl z)))
                  = (\<Sum>z\<in>UNIV. count_list (f z) (Inl y) * count_list xs (Inl z))
-                 + (\<Sum>z\<in>UNIV. if x = z then count_list (f z) (Inl y) else 0)" .
+                    + (\<Sum>z\<in>UNIV. if x = z then count_list (f z) (Inl y) else 0)" .
     then show "count_list (f x) (Inl y) + (\<Sum>z\<in>UNIV. count_list (f z) (Inl y) * count_list xs (Inl z)) 
             = (\<Sum>z\<in>UNIV. count_list (f z) (Inl y) * (if x = z then count_list xs (Inl z) + 1 
                                                               else count_list xs (Inl z)))"
-    proof (simp)
-    
-    (*have "(\<Sum>z\<in>UNIV. count_list (f z) (Inl y) * (if x = z then 1 else 0)) = count_list (f x) (Inl y)" *)
-
-(*
-  proof (simp)
-    let ?g = "(\<lambda>ba. if b = ba then count_list (f ba) a else 0)"
-    let ?h = "(\<lambda>ba. count_list (f ba) a * (count_list xs ba))"
-    have "sum (\<lambda>ba. count_list (f ba) a * (if b = ba then count_list xs ba + 1 else count_list xs ba)) UNIV =
-          sum (%x. ?g x + ?h x) UNIV"
-      by(rule cong[of "%f. sum f UNIV" "%f. sum f UNIV"], auto)
-    also have "sum (%x. ?g x + ?h x) UNIV = sum ?g UNIV + sum ?h UNIV"
-      by (rule sum.distrib)
-    finally have "sum (\<lambda>ba. count_list (f ba) a * (if b = ba then count_list xs ba + 1 else count_list xs ba)) UNIV
-             = sum ?g UNIV + sum ?h UNIV"
       by simp
-    thus "count_list (f b) a + count_list (concat (map f xs)) a
-        = sum (\<lambda>ba. count_list (f ba) a * (if b = ba then count_list xs ba + 1 else count_list xs ba)) UNIV"
-    proof (simp)
-      show "count_list (concat (map f xs)) a = (\<Sum>ba\<in>UNIV. count_list (f ba) a * count_list xs ba)"
-        by (rule Cons)
-    qed
   qed
-
-*)
 qed
 
 
-lemma assumes "single_use f" "single_use g"
-  shows "single_use (concat o (map f) o g)"
-  unfolding single_use_def bounded_def
+lemma
+  fixes f :: "('y::finite, 'z::finite, 'b) update'"
+  assumes "single_use f" and "single_use g"
+  shows "single_use (f \<bullet> g)"
+  unfolding bounded_def
 proof (rule allI)
-  have[rule_format, simp]: "\<forall>x y. count_list (g y) x \<le> Suc 0"
-  proof (intro  allI)
+  have[rule_format, simp]: "\<forall>x y. count_list (g y) (Inl x) \<le> Suc 0"
+  proof (intro allI)
     fix x y
-    show "count_list (g y) x \<le> Suc 0"
+    show "count_list (g y) (Inl x) \<le> Suc 0"
     proof (rule sumk[of UNIV y], auto)
       from assms
       have "count_var g x \<le> Suc 0"
-        by (simp add: single_use_def bounded_def)
-      thus "(\<Sum>a\<in>UNIV. count_list (g a) x) \<le> Suc 0"
+        by (simp add: bounded_def)
+      thus "(\<Sum>a\<in>UNIV. count_list (g a) (Inl x)) \<le> Suc 0"
         by (simp add: count_var_def)
     qed
   qed
-  fix x
-  show "count_var (concat \<circ> map f \<circ> g) x \<le> 1"
+  fix x :: "'z"
+  show "count_var (f \<bullet> g) x \<le> 1"
   proof (auto simp add: count_var_def)
     from assms
     have "count_var f x \<le> Suc 0"
-      by (simp add: single_use_def bounded_def)
-    hence "count_var f x = 0 \<or> count_var f x = Suc 0"
+      by (simp add:  bounded_def)
+    hence "count_var f x = 0 \<or> count_var f x = 1"
       by auto
-    thus "(\<Sum>y\<in>UNIV. count_list (concat (map f (g y))) x) \<le> Suc 0"
+    thus "(\<Sum>y\<in>UNIV. count_list ((f \<bullet> g) y) (Inl x)) \<le> Suc 0"
     proof
       assume "count_var f x = 0"
-      hence [simp]: "\<forall>y. count_list (f y) x = 0"
+      hence [simp]: "\<forall>y. count_list (f y) (Inl x) = 0"
         unfolding count_var_def
-        by(auto)
+        by (auto)
       show ?thesis
-        by (simp add: basic_count)
+        by (simp add: basic_count comp_def)
     next
-      assume a1: "count_var f x = Suc 0"
+      assume a1: "count_var f x = 1"
       show ?thesis
-      proof (simp add: basic_count)
-        have "\<exists>y \<in> UNIV. (%y. count_list (f y) x) y = 1 \<and> sum (%y. count_list (f y) x) (UNIV - {y}) = 0"
-          by(rule sum1, simp, insert a1, simp add: count_var_def)
-        then obtain z where z: "(%y. count_list (f y) x) z = 1"
-          "sum (%y. count_list (f y) x) (UNIV - {z}) = 0"
+      proof (simp add: comp_def basic_count)
+        have "\<exists>y \<in> UNIV. (\<lambda>y. count_list (f y) (Inl x)) y = 1 \<and> sum (\<lambda>y. count_list (f y) (Inl x)) (UNIV - {y}) = 0"
+          by (rule sum1, simp, insert a1, simp add: count_var_def)
+        then obtain z where z: "(\<lambda>y. count_list (f y) (Inl x)) z = Suc 0"
+          "sum (\<lambda>y. count_list (f y) (Inl x)) (UNIV - {z}) = 0"
           by auto
-        have "(\<Sum>y\<in>UNIV. \<Sum>b\<in>UNIV. count_list (f b) x * count_list (g y) b)
-            \<le> (\<Sum>y\<in>UNIV. count_list (g y) z)"
+        have "(\<Sum>y\<in>UNIV. \<Sum>b\<in>UNIV. count_list (f b) (Inl x) * count_list (g y) (Inl b))
+            \<le> (\<Sum>y\<in>UNIV. count_list (g y) (Inl z))"
         proof (rule sum_mono)
           fix y
-          have "(\<Sum>b\<in>UNIV. count_list (f b) x * count_list (g y) b) =
-                (\<Sum>b\<in>(insert z (UNIV - {z})). count_list (f b) x * count_list (g y) b)"
-            by(simp add: insert_UNIV)
-          also have "... = count_list (f z) x * count_list (g y) z +
-             (\<Sum>b\<in>(UNIV - {z}). count_list (f b) x * count_list (g y) b)"
+          have "(\<Sum>b\<in>UNIV. count_list (f b) (Inl x) * count_list (g y) (Inl b)) =
+                (\<Sum>b\<in>(insert z (UNIV - {z})). count_list (f b) (Inl x) * count_list (g y) (Inl b))"
+            by (simp add: insert_UNIV)
+          also have "... = count_list (f z) (Inl x) * count_list (g y) (Inl z) +
+             (\<Sum>b\<in>(UNIV - {z}). count_list (f b) (Inl x) * count_list (g y) (Inl b))"
             by (rule sum.insert, auto)
-          also have "... =  count_list (g y) z"
-            using z by(simp)
-          finally show "(\<Sum>b\<in>UNIV. count_list (f b) x * count_list (g y) b) \<le>
-            count_list (g y) z"
+          also have "... =  count_list (g y) (Inl z)"
+            using z by (simp)
+          finally show "(\<Sum>b\<in>UNIV. count_list (f b) (Inl x) * count_list (g y) (Inl b)) \<le>
+            count_list (g y) (Inl z)"
             by simp
         qed
         also have "... \<le> Suc 0"
-          using assms by (simp add: single_use_def bounded_def count_var_def)
-        finally show "(\<Sum>y\<in>UNIV. \<Sum>b\<in>UNIV. count_list (f b) x * count_list (g y) b) \<le> Suc 0"
+          using assms by (simp add: bounded_def count_var_def)
+        finally show "(\<Sum>y\<in>UNIV. \<Sum>b\<in>UNIV. count_list (f b) (Inl x) * count_list (g y) (Inl b)) \<le> Suc 0"
           by simp
       qed
     qed
